RBT.v
@@ -1,0 +1,1973 @@
+
+(** * MMaps.RBT *)
+
+(** This module implements finite maps using Red-Black trees.
+    This code is based on [MSetRBT.v], due initially to
+    Andrew W. Appel, 2011. See initial comment at the beginning
+    of [MSetRBT.v].
+
+    Note that we only prove here that the operations below preserve
+    the binary search tree invariant ([Bst], a.k.a [Ok] predicate here),
+    but *not* the Red/Black balancing invariant. Indeed, the former
+    is enough to implement the desired interface [S], and ensure
+    observational correctness. And proceeding this way is much lighter.
+
+    Of course, the Red/Black invariants are also meant to be preserved
+    here (otherwise we could end with wrong complexities). It shouldn't
+    be too hard to adapt the proofs of [MSetRBT.BalanceProps] to this
+    file, but this remains to be done.
+*)
+
+From Coq Require Import Bool BinPos Pnat Setoid SetoidList PeanoNat.
+From Coq Require Import Orders OrdersFacts OrdersLists.
+From MMaps Require Import Interface OrdList GenTree.
+
+Local Set Implicit Arguments.
+Local Unset Strict Implicit.
+Import ListNotations.
+
+(* For nicer extraction, we create inductive principles
+   only when needed *)
+Local Unset Elimination Schemes.
+
+(** Notations and helper lemma about pairs *)
+
+Notation "s #1" := (fst s) (at level 9, format "s '#1'") : pair_scope.
+Notation "s #2" := (snd s) (at level 9, format "s '#2'") : pair_scope.
+
+(** The type of color annotation. *)
+
+Inductive color := Red | Black.
+
+Module Color.
+ Definition t := color.
+End Color.
+
+(** * The Raw functor
+
+   Functor of pure functions + separate proofs of invariant
+   preservation *)
+
+Module Raw (K: OrderedType).
+
+(** ** Generic trees instantiated with Red/Black colors *)
+
+(** We reuse a generic definition of trees where the information
+    parameter is a [Color.t]. Functions like mem or fold are also
+    provided by this generic functor. *)
+
+Include MMaps.GenTree.Ops K Color.
+
+Local Open Scope pair_scope.
+Local Open Scope lazy_bool_scope.
+Local Notation color := Color.t.
+Local Arguments Leaf {elt}.
+Local Notation Rd := (@Node _ Red).
+Local Notation Bk := (@Node _ Black).
+
+Section Elt.
+Variable elt : Type.
+Local Notation t := (tree elt).
+Implicit Types l r m : t.
+Implicit Types e : elt.
+
+(** ** Basic tree *)
+
+Definition singleton (k : key) (v : elt) : t :=
+  Node Black Leaf k v Leaf.
+
+(** ** Changing root color *)
+
+Definition makeBlack m : t :=
+ match m with
+ | Leaf => Leaf
+ | Node _ a x v b => Bk a x v b
+ end.
+
+Definition makeRed m : t :=
+ match m with
+ | Leaf => Leaf
+ | Node _ a x v b => Rd a x v b
+ end.
+
+(** ** Balancing *)
+
+(** We adapt when one side is not a true red-black tree.
+    Both sides have the same black depth. *)
+
+Definition lbal l k vk r :=
+ match l with
+ | Rd (Rd a x vx b) y vy c => Rd (Bk a x vx b) y vy (Bk c k vk r)
+ | Rd a x vx (Rd b y vy c) => Rd (Bk a x vx b) y vy (Bk c k vk r)
+ | _ => Bk l k vk r
+ end.
+
+Definition rbal l k vk r :=
+ match r with
+ | Rd (Rd b y vy c) z vz d => Rd (Bk l k vk b) y vy (Bk c z vz d)
+ | Rd b y vy (Rd c z vz d) => Rd (Bk l k vk b) y vy (Bk c z vz d)
+ | _ => Bk l k vk r
+ end.
+
+(** A variant of [rbal], with reverse pattern order. *)
+
+Definition rbal' l k vk r :=
+ match r with
+ | Rd b y vy (Rd c z vz d) => Rd (Bk l k vk b) y vy (Bk c z vz d)
+ | Rd (Rd b y vy c) z vz d => Rd (Bk l k vk b) y vy (Bk c z vz d)
+ | _ => Bk l k vk r
+ end.
+
+(** Balancing with different black depth.
+    One side is almost a red-black tree, while the other is
+    a true red-black tree, but with black depth + 1.
+    Used in deletion. *)
+
+Definition lbalS l k vk r :=
+ match l with
+ | Rd a x vx b => Rd (Bk a x vx b) k vk r
+ | _ =>
+   match r with
+   | Bk a y vy b => rbal' l k vk (Rd a y vy b)
+   | Rd (Bk a y vy b) z vz c => Rd (Bk l k vk a) y vy (rbal' b z vz (makeRed c))
+   | _ => Rd l k vk r (* impossible *)
+   end
+ end.
+
+Definition rbalS l k vk r :=
+ match r with
+ | Rd b y vy c => Rd l k vk (Bk b y vy c)
+ | _ =>
+   match l with
+   | Bk a x vx b => lbal (Rd a x vx b) k vk r
+   | Rd a x vx (Bk b y vy c) => Rd (lbal (makeRed a) x vx b) y vy (Bk c k vk r)
+   | _ => Rd l k vk r (* impossible *)
+   end
+ end.
+
+(** ** Insertion *)
+
+Fixpoint ins x vx s :=
+ match s with
+ | Leaf => Rd Leaf x vx Leaf
+ | Node c l y vy r =>
+   match K.compare x y with
+   | Eq => Node c l y vx r
+   | Lt =>
+     match c with
+     | Red => Rd (ins x vx l) y vy r
+     | Black => lbal (ins x vx l) y vy r
+     end
+   | Gt =>
+     match c with
+     | Red => Rd l y vy (ins x vx r)
+     | Black => rbal l y vy (ins x vx r)
+     end
+   end
+ end.
+
+Definition add x vx s := makeBlack (ins x vx s).
+
+(** ** Deletion *)
+
+Fixpoint append (l:t) : t -> t :=
+ match l with
+ | Leaf => fun r => r
+ | Node lc ll lx lv lr =>
+   fix append_l (r:t) : t :=
+   match r with
+   | Leaf => l
+   | Node rc rl rx rv rr =>
+     match lc, rc with
+     | Red, Red =>
+       let lrl := append lr rl in
+       match lrl with
+       | Rd lr' x v rl' => Rd (Rd ll lx lv lr') x v (Rd rl' rx rv rr)
+       | _ => Rd ll lx lv (Rd lrl rx rv rr)
+       end
+     | Black, Black =>
+       let lrl := append lr rl in
+       match lrl with
+       | Rd lr' x v rl' => Rd (Bk ll lx lv lr') x v (Bk rl' rx rv rr)
+       | _ => lbalS ll lx lv (Bk lrl rx rv rr)
+       end
+     | Black, Red => Rd (append_l rl) rx rv rr
+     | Red, Black => Rd ll lx lv (append lr r)
+     end
+   end
+ end.
+
+Fixpoint del x m : t :=
+ match m with
+ | Leaf => Leaf
+ | Node _ a y v b =>
+   match K.compare x y with
+   | Eq => append a b
+   | Lt =>
+     match a with
+     | Bk _ _ _ _ => lbalS (del x a) y v b
+     | _ => Rd (del x a) y v b
+     end
+   | Gt =>
+     match b with
+     | Bk _ _ _ _ => rbalS a y v (del x b)
+     | _ => Rd a y v (del x b)
+     end
+   end
+ end.
+
+Definition remove x m := makeBlack (del x m).
+
+(** ** Tree-ification
+
+    We rebuild a tree of size [if pred then n-1 else n] as soon
+    as the list [l] has enough elements *)
+
+Definition klist A := list (key * A).
+Local Notation treeify_t := (klist elt -> t * klist elt).
+
+Definition bogus : t * klist elt := (Leaf, nil).
+
+Definition treeify_zero : treeify_t :=
+ fun acc => (Leaf,acc).
+
+Definition treeify_one : treeify_t :=
+ fun acc => match acc with
+ | (x,v)::acc => (Rd Leaf x v Leaf, acc)
+ | _ => bogus
+ end.
+
+Definition treeify_cont (f g : treeify_t) : treeify_t :=
+ fun acc =>
+ match f acc with
+ | (l, (x,v)::acc) =>
+   match g acc with
+   | (r, acc) => (Bk l x v r, acc)
+   end
+ | _ => bogus
+ end.
+
+Fixpoint treeify_aux (pred:bool)(n: positive) : treeify_t :=
+ match n with
+ | xH => if pred then treeify_zero else treeify_one
+ | xO n => treeify_cont (treeify_aux pred n) (treeify_aux true n)
+ | xI n => treeify_cont (treeify_aux false n) (treeify_aux pred n)
+ end.
+
+Fixpoint plength_aux (l:klist elt)(p:positive) := match l with
+ | nil => p
+ | _::l => plength_aux l (Pos.succ p)
+end.
+
+Definition plength (l:klist elt) := plength_aux l 1.
+
+Definition treeify (l:klist elt) :=
+ fst (treeify_aux true (plength l) l).
+
+End Elt.
+
+(** * Map with removal *)
+
+Definition ocons {A B} (a:A) (o:option B) (l:list (A*B)) :=
+ match o with
+ | None => l
+ | Some b => (a,b)::l
+ end.
+
+Section Mapo.
+Variable elt elt' : Type.
+Variable f : key -> elt -> option elt'.
+
+Fixpoint mapoL (l : klist elt)(acc : klist elt') : klist elt' :=
+  match l with
+   | nil => acc
+   | (k,v)::l => mapoL l (ocons k (f k v) acc)
+  end.
+
+Definition mapo (m : t elt) : t elt' :=
+ treeify (mapoL (rev_bindings m) nil).
+
+End Mapo.
+
+(** * Merge *)
+
+Section Merge.
+Variable elt elt' elt'' : Type.
+Variable f : key -> option elt -> option elt' -> option elt''.
+
+Fixpoint mergeL (l1:klist elt) :
+ klist elt' -> klist elt'' -> klist elt'' :=
+ match l1 with
+ | nil => mapoL (fun k v' => f k None (Some v'))
+ | (x,vx)::l1' =>
+    fix mergeL_l1 l2 acc :=
+    match l2 with
+    | nil => mapoL (fun k v => f k (Some v) None) l1 acc
+    | (y,vy)::l2' =>
+       match K.compare x y with
+       | Eq => mergeL l1' l2' (ocons x (f x (Some vx) (Some vy)) acc)
+       | Lt => mergeL_l1 l2' (ocons y (f y None (Some vy)) acc)
+       | Gt => mergeL l1' l2 (ocons x (f x (Some vx) None) acc)
+       end
+    end
+ end.
+
+Definition merge (m1 : t elt) (m2 : t elt') : t elt'' :=
+ treeify (mergeL (rev_bindings m1) (rev_bindings m2) nil).
+
+End Merge.
+
+(** * Correctness proofs *)
+
+Include MMaps.GenTree.Props K Color.
+
+Local Infix "∈" := In (at level 70).
+Local Infix "==" := K.eq (at level 70).
+Local Infix "<" := K.lt (at level 70).
+Local Infix "<<" := Below (at level 70).
+Local Infix ">>" := Above (at level 70).
+Local Infix "<<<" := Apart (at level 70).
+Local Infix "===" := Equal (at level 70).
+
+Local Hint Constructors tree MapsTo In Bst Above Below.
+Local Hint Unfold In0 Apart Ok Bst_Ok.
+Local Hint Immediate F.eq_sym.
+Local Hint Resolve F.eq_refl F.eq_trans F.lt_trans.
+Local Hint Resolve
+ AboveLt Above_not_In Above_trans
+ BelowGt Below_not_In Below_trans.
+
+Ltac chok := change Bst with Ok in *.
+Ltac autok := chok; auto with typeclass_instances.
+Ltac ok :=
+ match goal with
+   | H : Ok (Node _ _ _ _ _) |- _ => inversion_clear H; chok; ok
+   | H : Above _ (Node _ _ _ _ _) |- _ => inversion_clear H; ok
+   | H : Below _ (Node _ _ _ _ _) |- _ => inversion_clear H; ok
+   | |- Ok (Node _ _ _ _ _) => constructor; autok; ok
+   | |- Above _ (Node _ _ _ _ _) => constructor; ok
+   | |- Below _ (Node _ _ _ _ _) => constructor; ok
+   | _ => eauto with typeclass_instances
+ end.
+
+Ltac induct m :=
+ induction m as [|c l IHl x' vx' r IHr]; simpl; intros;
+ [|case K.compare_spec; intros; inv Ok; chok].
+
+Ltac destmatch :=
+ match goal with
+ | |- context [match K.compare _ _ with _ => _ end] =>
+   case K.compare_spec; destmatch
+ | |- context [match ?x with _ => _ end] =>
+   destruct x; destmatch
+ | _ => idtac
+ end.
+
+Section Elt.
+Variable elt : Type.
+Implicit Types m : t elt.
+Implicit Types k x y : key.
+Implicit Types v vx vy : elt.
+
+(** ** Singleton set *)
+
+Lemma singleton_spec x y vx vy :
+  MapsTo y vy (singleton x vx) <-> y == x /\ vy = vx.
+Proof.
+ unfold singleton; intuition_in. subst; auto.
+Qed.
+
+Global Instance singleton_ok x vx : Ok (singleton x vx).
+Proof.
+ unfold singleton. ok.
+Qed.
+
+(** ** makeBlack, MakeRed *)
+
+Global Instance makeBlack_ok m `{!Ok m} : Ok (makeBlack m).
+Proof.
+ destruct m; simpl; ok.
+Qed.
+
+Global Instance makeRed_ok m `{!Ok m} : Ok (makeRed m).
+Proof.
+ destruct m; simpl; ok.
+Qed.
+
+Lemma makeBlack_in m x : In x (makeBlack m) <-> In x m.
+Proof.
+ destruct m; simpl; intuition_in.
+Qed.
+
+Lemma makeRed_in m x : In x (makeRed m) <-> In x m.
+Proof.
+ destruct m; simpl; intuition_in.
+Qed.
+
+Lemma makeBlack_mapsto m x v : MapsTo x v (makeBlack m) <-> MapsTo x v m.
+Proof.
+ destruct m; simpl; intuition_in.
+Qed.
+
+Lemma makeRed_mapsto m x v : MapsTo x v (makeRed m) <-> MapsTo x v m.
+Proof.
+ destruct m; simpl; intuition_in.
+Qed.
+
+Lemma makeBlack_find m : makeBlack m === m.
+Proof.
+ now destruct m.
+Qed.
+
+Lemma makeRed_find m : makeRed m === m.
+Proof.
+ now destruct m.
+Qed.
+
+(** ** Generic handling for red-matching and red-red-matching *)
+
+Definition isblack m :=
+ match m with Bk _ _ _ _ => True | _ => False end.
+
+Definition notblack m :=
+ match m with Bk _ _ _ _ => False | _ => True end.
+
+Definition notred m :=
+ match m with Rd _ _ _ _ => False | _ => True end.
+
+Definition rcase {A} f g m : A :=
+ match m with
+ | Rd a x v b => f a x v b
+ | _ => g m
+ end.
+
+Inductive rspec {A} f g : t elt -> A -> Prop :=
+ | rred a x v b : rspec f g (Rd a x v b) (f a x v b)
+ | relse t : notred t -> rspec f g t (g t).
+
+Fact rmatch {A} f g m : rspec (A:=A) f g m (rcase f g m).
+Proof.
+unfold rcase. destmatch; now constructor.
+Qed.
+
+Definition rrcase {A} f g m : A :=
+ match m with
+ | Rd (Rd a x vx b) y vy c => f a x vx b y vy c
+ | Rd a x vx (Rd b y vy c) => f a x vx  b y vy c
+ | _ => g m
+ end.
+
+Notation notredred := (rrcase (fun _ _ _ _ _ _ _ => False) (fun _ => True)).
+
+Inductive rrspec {A} f g : t elt -> A -> Prop :=
+ | rrleft a x vx b y vy c :
+     rrspec f g (Rd (Rd a x vx b) y vy c) (f a x vx b y vy c)
+ | rrright a x vx b y vy c :
+     rrspec f g (Rd a x vx (Rd b y vy c)) (f a x vx b y vy c)
+ | rrelse m : notredred m -> rrspec f g m (g m).
+
+Fact rrmatch {A} f g m : rrspec (A:=A) f g m (rrcase f g m).
+Proof.
+unfold rrcase. destmatch; now constructor.
+Qed.
+
+Definition rrcase' {A} f g m : A :=
+ match m with
+ | Rd a x vx (Rd b y vy c) => f a x vx b y vy c
+ | Rd (Rd a x vx b) y vy c => f a x vx b y vy c
+ | _ => g m
+ end.
+
+Fact rrmatch' {A} f g m : rrspec (A:=A) f g m (rrcase' f g m).
+Proof.
+unfold rrcase'. destmatch; now constructor.
+Qed.
+
+(** Balancing operations are instances of generic match *)
+
+Fact lbal_match l k v r :
+ rrspec
+   (fun a x vx b y vy c => Rd (Bk a x vx b) y vy (Bk c k v r))
+   (fun l => Bk l k v r)
+   l
+   (lbal l k v r).
+Proof.
+ exact (rrmatch _ _ _).
+Qed.
+
+Fact rbal_match l k v r :
+ rrspec
+   (fun a x vx b y vy c => Rd (Bk l k v a) x vx (Bk b y vy c))
+   (fun r => Bk l k v r)
+   r
+   (rbal l k v r).
+Proof.
+ exact (rrmatch _ _ _).
+Qed.
+
+Fact rbal'_match l k v r :
+ rrspec
+   (fun a x vx b y vy c => Rd (Bk l k v a) x vx (Bk b y vy c))
+   (fun r => Bk l k v r)
+   r
+   (rbal' l k v r).
+Proof.
+ exact (rrmatch' _ _ _).
+Qed.
+
+Fact lbalS_match l x vx r :
+ rspec
+  (fun a y vy b => Rd (Bk a y vy b) x vx r)
+  (fun l =>
+    match r with
+    | Bk a y vy b => rbal' l x vx (Rd a y vy b)
+    | Rd (Bk a y vy b) z vz c =>
+      Rd (Bk l x vx a) y vy (rbal' b z vz (makeRed c))
+    | _ => Rd l x vx r
+    end)
+  l
+  (lbalS l x vx r).
+Proof.
+ exact (rmatch _ _ _).
+Qed.
+
+Fact rbalS_match l x vx r :
+ rspec
+  (fun a y vy b => Rd l x vx (Bk a y vy b))
+  (fun r =>
+    match l with
+    | Bk a y vy b => lbal (Rd a y vy b) x vx r
+    | Rd a y vy (Bk b z vz c) =>
+      Rd (lbal (makeRed a) y vy b) z vz (Bk c x vx r)
+    | _ => Rd l x vx r
+    end)
+  r
+  (rbalS l x vx r).
+Proof.
+ exact (rmatch _ _ _).
+Qed.
+
+(** ** Balancing for insertion *)
+
+Global Instance lbal_ok l x v r `(!Ok l, !Ok r, x >> l, x << r) :
+ Ok (lbal l x v r).
+Proof.
+ destruct (lbal_match l x v r); ok.
+Qed.
+
+Lemma lbal_in l x v r y :
+ In y (lbal l x v r) <-> K.eq y x \/ In y l \/ In y r.
+Proof.
+ case lbal_match; intuition_in.
+Qed.
+
+(** Note : Rd is arbitrary here and in all similar results below *)
+
+Lemma lbal_mapsto l x vx r y vy :
+ MapsTo y vy (lbal l x vx r) <-> MapsTo y vy (Rd l x vx r).
+Proof.
+ case lbal_match; intuition_in.
+Qed.
+
+Lemma lbal_find l x v r `{!Ok l, !Ok r} :
+ x >> l -> x << r ->
+ lbal l x v r === Rd l x v r.
+Proof.
+ intros. intro. apply find_mapsto_equiv; auto using lbal_mapsto; autok.
+Qed.
+
+Global Instance rbal_ok l x v r `(!Ok l, !Ok r, x >> l, x << r) :
+ Ok (rbal l x v r).
+Proof.
+ destruct (rbal_match l x v r); ok.
+Qed.
+
+Lemma rbal_in l x v r y :
+ In y (rbal l x v r) <-> K.eq y x \/ In y l \/ In y r.
+Proof.
+ case rbal_match; intuition_in.
+Qed.
+
+Lemma rbal_mapsto l x vx r y vy :
+ MapsTo y vy (rbal l x vx r) <-> MapsTo y vy (Rd l x vx r).
+Proof.
+ case rbal_match; intuition_in.
+Qed.
+
+Lemma rbal_find l x v r `{!Ok l, !Ok r} :
+ x >> l -> x << r ->
+ rbal l x v r === Rd l x v r.
+Proof.
+ intros. intro. apply find_mapsto_equiv; auto using rbal_mapsto; autok.
+Qed.
+
+Global Instance rbal'_ok l x v r `(!Ok l, !Ok r, x >> l, x << r) :
+ Ok (rbal' l x v r).
+Proof.
+ destruct (rbal'_match l x v r); ok.
+Qed.
+
+Lemma rbal'_in l x r v y :
+ In y (rbal' l x v r) <-> K.eq y x \/ In y l \/ In y r.
+Proof.
+ case rbal'_match; intuition_in.
+Qed.
+
+Lemma rbal'_mapsto l x vx r y vy :
+ MapsTo y vy (rbal' l x vx r) <-> MapsTo y vy (Rd l x vx r).
+Proof.
+ case rbal'_match; intuition_in.
+Qed.
+
+Lemma rbal'_find l x v r `{!Ok l, !Ok r} :
+ x >> l -> x << r ->
+ rbal' l x v r === Rd l x v r.
+Proof.
+ intros. intro. apply find_mapsto_equiv; auto using rbal'_mapsto; autok.
+Qed.
+
+Hint Rewrite (@In_node_iff elt)
+ makeRed_in makeBlack_in lbal_in rbal_in rbal'_in : rb.
+
+Ltac autorew := autorewrite with rb.
+Tactic Notation "autorew" "in" ident(H) := autorewrite with rb in H.
+Ltac treeorder :=
+ rewrite ?below_alt, ?above_alt; try intro; autorew; intuition_in; order.
+
+(** ** Insertion *)
+
+Lemma ins_in m x v y :
+ In y (ins x v m) <-> K.eq y x \/ In y m.
+Proof.
+ induct m; destmatch; autorew; rewrite ?IHl, ?IHr; intuition_in.
+ setoid_replace y with x; eauto.
+Qed.
+Hint Rewrite ins_in : rb.
+
+Lemma ins_above m x v y : y >> m -> x < y -> y >> ins x v m.
+Proof.
+ intros. treeorder.
+Qed.
+
+Lemma ins_below m x v y : y << m -> y < x -> y << ins x v m.
+Proof.
+ intros. treeorder.
+Qed.
+Hint Resolve ins_above ins_below.
+
+Global Instance ins_ok m x v `{!Ok m} : Ok (ins x v m).
+Proof.
+ induct m; auto; destmatch;
+ (eapply lbal_ok || eapply rbal_ok || ok); auto.
+Qed.
+
+Lemma ins_spec1 m x v `{!Ok m} : find x (ins x v m) = Some v.
+Proof.
+ induct m; simpl; destmatch;
+  rewrite ?lbal_find, ?rbal_find by eauto with *;
+  simpl; destmatch; auto; try order.
+Qed.
+
+Lemma ins_spec2 m x y v `{!Ok m} : ~ x == y ->
+ find y (ins x v m) = find y m.
+Proof.
+ induct m; simpl; destmatch;
+  rewrite ?lbal_find, ?rbal_find by eauto with *;
+  simpl; destmatch; auto; try order.
+Qed.
+
+Lemma ins_find m x y v `{!Ok m} :
+ find y (ins x v m) =
+  match K.compare y x with Eq => Some v | _ => find y m end.
+Proof.
+ destmatch; intros E.
+ - apply find_spec; autok. rewrite E. apply find_spec; autok.
+   now apply ins_spec1.
+ - apply ins_spec2; trivial; order.
+ - apply ins_spec2; trivial; order.
+Qed.
+
+Global Instance add_ok m x v `{!Ok m} : Ok (add x v m).
+Proof.
+ unfold add; autok.
+Qed.
+
+Lemma add_in m x v y :
+ In y (add x v m) <-> K.eq y x \/ In y m.
+Proof.
+ unfold add. now autorew.
+Qed.
+Hint Rewrite add_in : rb.
+
+Lemma add_spec1 m x v `{!Ok m} : find x (add x v m) = Some v.
+Proof.
+unfold add. rewrite makeBlack_find. now apply ins_spec1.
+Qed.
+
+Lemma add_spec2 m x y v `{!Ok m} : ~ x == y ->
+ find y (add x v m) = find y m.
+Proof.
+unfold add. rewrite makeBlack_find. now apply ins_spec2.
+Qed.
+
+
+(** ** Balancing for deletion *)
+
+Lemma lbalS_in l x v r y :
+  In y (lbalS l x v r) <-> K.eq y x \/ In y l \/ In y r.
+Proof.
+ case lbalS_match.
+ - intros; autorew; intuition_in.
+ - clear l. intros l _. destmatch; autorew; intuition_in.
+Qed.
+
+Global Instance lbalS_ok l x v r :
+  forall `(!Ok l, !Ok r, x >> l, x << r), Ok (lbalS l x v r).
+Proof.
+ case lbalS_match; intros; destmatch; ok; try apply rbal'_ok; treeorder.
+Qed.
+
+Lemma lbalS_mapsto l x v r y vy :
+  MapsTo y vy (lbalS l x v r) <-> MapsTo y vy (Rd l x v r).
+Proof.
+ case lbalS_match; intros.
+ - intuition_in.
+ - destmatch; intuition_in;
+   rewrite ?rbal'_mapsto in *; intuition_in;
+   rewrite ?makeRed_mapsto in *; intuition_in;
+   apply MapsRight; rewrite rbal'_mapsto; intuition_in.
+   apply MapsRight. now rewrite makeRed_mapsto.
+Qed.
+
+Lemma lbalS_find l x v r `{!Ok l, !Ok r} : x >> l -> x << r ->
+  lbalS l x v r === Rd l x v r.
+Proof.
+ intros. intro. apply find_mapsto_equiv; auto using lbalS_mapsto; autok.
+Qed.
+
+Lemma rbalS_in l x r v y :
+  In y (rbalS l x v r) <-> K.eq y x \/ In y l \/ In y r.
+Proof.
+ case rbalS_match.
+ - intuition_in.
+ - intros t _. destmatch; autorew; intuition_in.
+Qed.
+
+Global Instance rbalS_ok l x v r :
+ forall `(!Ok l, !Ok r, x >> l, x << r), Ok (rbalS l x v r).
+Proof.
+ case rbalS_match; intros; destmatch; ok; try (apply lbal_ok); treeorder.
+Qed.
+
+Lemma rbalS_mapsto l x v r y vy :
+  MapsTo y vy (rbalS l x v r) <-> MapsTo y vy (Rd l x v r).
+Proof.
+ case rbalS_match; intros.
+ - intuition_in.
+ - destmatch; intuition_in;
+   rewrite ?lbal_mapsto in *; intuition_in;
+   rewrite ?makeRed_mapsto in *; intuition_in;
+   apply MapsLeft; rewrite lbal_mapsto; intuition_in.
+   apply MapsLeft. now rewrite makeRed_mapsto.
+Qed.
+
+Lemma rbalS_find l x v r `{!Ok l, !Ok r} : x >> l -> x << r ->
+  rbalS l x v r === Rd l x v r.
+Proof.
+ intros. intro. apply find_mapsto_equiv; auto using rbalS_mapsto; autok.
+Qed.
+
+Hint Rewrite lbalS_in rbalS_in : rb.
+
+(** ** Append for deletion *)
+
+Ltac append_tac l r :=
+ induction l as [| lc ll _ lx lv lr IHlr];
+ [intro r; simpl
+ |induction r as [| rc rl IHrl rx rv rr _];
+   [simpl
+   |destruct lc, rc;
+     [specialize (IHlr rl); clear IHrl
+     |simpl;
+      assert (Hr:notred (Bk rl rx rv rr)) by (simpl; trivial);
+      set (r:=Bk rl rx rv rr) in *; clearbody r; clear IHrl rl rx rv rr;
+      specialize (IHlr r)
+     |change (append _ _) with (Rd (append (Bk ll lx lv lr) rl) rx rv rr);
+      assert (Hl:notred (Bk ll lx lv lr)) by (simpl; trivial);
+      set (l:=Bk ll lx lv lr) in *; clearbody l; clear IHlr ll lx lv lr
+     |specialize (IHlr rl); clear IHrl]]].
+
+Fact append_rr_match ll lx lv lr rl rx rv rr :
+ rspec
+  (fun a x v b => Rd (Rd ll lx lv a) x v (Rd b rx rv rr))
+  (fun t => Rd ll lx lv (Rd t rx rv rr))
+  (append lr rl)
+  (append (Rd ll lx lv lr) (Rd rl rx rv rr)).
+Proof.
+ exact (rmatch _ _ _).
+Qed.
+
+Fact append_bb_match ll lx lv lr rl rx rv rr :
+ rspec
+  (fun a x v b => Rd (Bk ll lx lv a) x v (Bk b rx rv rr))
+  (fun t => lbalS ll lx lv (Bk t rx rv rr))
+  (append lr rl)
+  (append (Bk ll lx lv lr) (Bk rl rx rv rr)).
+Proof.
+ exact (rmatch _ _ _).
+Qed.
+
+Lemma append_in l r x :
+ In x (@append elt l r) <-> In x l \/ In x r.
+Proof.
+ revert r.
+ append_tac l r; autorew; try (intuition_in; fail).
+ - (* Red / Red *)
+   revert IHlr; case append_rr_match;
+    [intros a y v b | intros t Ht]; autorew; tauto.
+ - (* Black / Black *)
+   revert IHlr; case append_bb_match;
+    [intros a y v b | intros t Ht]; autorew; tauto.
+Qed.
+
+Hint Rewrite append_in : rb.
+
+Global Instance append_ok : forall l r `{!Ok l, !Ok r},
+ l <<< r -> Ok (@append elt l r).
+Proof.
+ append_tac l r; trivial; intros OK OK' AP;
+ rewrite ?apart_node_l, ?apart_node_r in AP;
+ decompose [and] AP; clear AP; ok; try treeorder.
+ - (* Rd / Rd *)
+   assert (U : Ok (append lr rl)) by auto.
+   assert (V : lx << append lr rl) by treeorder.
+   assert (W : rx >> append lr rl) by treeorder.
+   revert U V W; case append_rr_match; intros; ok.
+ - (* Bk / Bk *)
+   assert (U : Ok (append lr rl)) by auto.
+   assert (V : lx << append lr rl) by treeorder.
+   assert (W : rx >> append lr rl) by treeorder.
+   revert U V W; case append_bb_match; intros; ok.
+Qed.
+
+Lemma append_mapsto l r y v :
+  MapsTo y v (append l r) <-> MapsTo y v l \/ MapsTo y v r.
+Proof.
+ revert r.
+ append_tac l r; try (intuition_in; fail).
+ - (* Rd / Rd *)
+   simpl; intros.
+   destmatch; revert IHlr; rewrite !MapsTo_node_iff; intuition.
+ - (* Bk / Bk *)
+   simpl; intros.
+   destmatch; revert IHlr;
+    rewrite ?lbalS_mapsto, !MapsTo_node_iff; intuition.
+Qed.
+
+(** ** Deletion *)
+
+Lemma del_in m x y `{!Ok m} :
+ In y (del x m) <-> In y m /\ ~K.eq y x.
+Proof.
+induct m; destmatch; treeorder.
+Qed.
+
+Hint Rewrite del_in : rb.
+
+Global Instance del_ok m x `{!Ok m} : Ok (del x m).
+Proof.
+induct m.
+- trivial.
+- eapply append_ok; eauto.
+- assert (x' >> del x l) by treeorder.
+  destmatch; ok.
+- assert (x' << del x r) by treeorder.
+  destmatch; ok.
+Qed.
+
+Lemma del_spec1 m x `{!Ok m} : find x (del x m) = None.
+Proof.
+apply not_find_iff; ok. rewrite del_in; treeorder.
+Qed.
+
+Lemma del_spec2 m x y `{!Ok m} : ~ x == y ->
+ find y (del x m) = find y m.
+Proof.
+intros.
+apply find_mapsto_equiv; ok.
+induct m.
+- easy.
+- rewrite append_mapsto, MapsTo_node_iff. treeorder.
+- destmatch.
+  + simpl. intuition_in.
+  + rewrite 2 MapsTo_node_iff. factornode l. now rewrite IHl by ok.
+  + rewrite lbalS_mapsto, 2 MapsTo_node_iff. factornode l.
+    now rewrite IHl by ok.
+- destmatch.
+  + simpl. intuition_in.
+  + rewrite 2 MapsTo_node_iff. factornode r. now rewrite IHr by ok.
+  + rewrite rbalS_mapsto, 2 MapsTo_node_iff. factornode r.
+    now rewrite IHr by ok.
+Qed.
+
+Lemma remove_in m x y `{!Ok m} :
+ In y (remove x m) <-> In y m /\ ~K.eq y x.
+Proof.
+unfold remove. now autorew.
+Qed.
+
+Hint Rewrite remove_in : rb.
+
+Global Instance remove_ok m x `{!Ok m} : Ok (remove x m).
+Proof.
+unfold remove; ok.
+Qed.
+
+Lemma remove_spec1 m x `{!Ok m} : find x (remove x m) = None.
+Proof.
+unfold remove. rewrite makeBlack_find. now apply del_spec1.
+Qed.
+
+Lemma remove_spec2 m x y `{!Ok m} : ~ x == y ->
+ find y (remove x m) = find y m.
+Proof.
+unfold remove. rewrite makeBlack_find. now apply del_spec2.
+Qed.
+
+(** ** Treeify *)
+
+Local Notation ifpred p n := (if p then pred n else n%nat).
+Local Notation treeify_t := (klist elt -> t elt * klist elt).
+
+Definition treeify_invariant size (f:treeify_t) :=
+ forall acc,
+ size <= length acc ->
+ let (m,acc') := f acc in
+ cardinal m = size /\ acc = bindings m ++ acc'.
+
+Lemma treeify_zero_spec : treeify_invariant 0 (@treeify_zero elt).
+Proof.
+ intro. simpl. auto.
+Qed.
+
+Lemma treeify_one_spec : treeify_invariant 1 (@treeify_one elt).
+Proof.
+ intros [|x acc]; simpl; auto. inversion 1.
+ destruct x. simpl; auto.
+Qed.
+
+Lemma treeify_cont_spec f g size1 size2 size :
+ treeify_invariant size1 f ->
+ treeify_invariant size2 g ->
+ size = S (size1 + size2) ->
+ treeify_invariant size (treeify_cont f g).
+Proof.
+ intros Hf Hg EQ acc LE. unfold treeify_cont.
+ specialize (Hf acc).
+ destruct (f acc) as (t1,acc1).
+ destruct Hf as (Hf1,Hf2).
+  { transitivity size; trivial. subst. auto with arith. }
+ destruct acc1 as [|x acc1].
+  { exfalso. revert LE. apply Nat.lt_nge. subst.
+    rewrite app_nil_r, <- bindings_cardinal; auto with arith. }
+ specialize (Hg acc1).
+ destruct (g acc1) as (t2,acc2).
+ destruct Hg as (Hg1,Hg2).
+  { revert LE. subst.
+    rewrite app_length, <- bindings_cardinal. simpl.
+    rewrite Nat.add_succ_r, <- Nat.succ_le_mono.
+    apply Nat.add_le_mono_l. }
+ destruct x; simpl.
+ rewrite bindings_node_acc. subst; auto.
+Qed.
+
+Lemma treeify_aux_spec n (p:bool) :
+ treeify_invariant (ifpred p (Pos.to_nat n)) (treeify_aux p n).
+Proof.
+ revert p.
+ induction n as [n|n|]; intros p; simpl treeify_aux.
+ - eapply treeify_cont_spec; [ apply (IHn false) | apply (IHn p) | ].
+   rewrite Pos2Nat.inj_xI.
+   assert (H := Pos2Nat.is_pos n). apply Nat.neq_0_lt_0 in H.
+   destruct p; simpl; intros; rewrite Nat.add_0_r; trivial.
+   now rewrite <- Nat.add_succ_r, Nat.succ_pred; trivial.
+ - eapply treeify_cont_spec; [ apply (IHn p) | apply (IHn true) | ].
+   rewrite Pos2Nat.inj_xO.
+   assert (H := Pos2Nat.is_pos n). apply Nat.neq_0_lt_0 in H.
+   rewrite <- Nat.add_succ_r, Nat.succ_pred by trivial.
+   destruct p; simpl; intros; rewrite Nat.add_0_r; trivial.
+   symmetry. now apply Nat.add_pred_l.
+ - destruct p; [ apply treeify_zero_spec | apply treeify_one_spec ].
+Qed.
+
+Lemma plength_aux_spec l p :
+  Pos.to_nat (@plength_aux elt l p) = length l + Pos.to_nat p.
+Proof.
+ revert p. induction l; trivial. simpl plength_aux.
+ intros. now rewrite IHl, Pos2Nat.inj_succ, Nat.add_succ_r.
+Qed.
+
+Lemma plength_spec l : Pos.to_nat (@plength elt l) = S (length l).
+Proof.
+ unfold plength. rewrite plength_aux_spec. apply Nat.add_1_r.
+Qed.
+
+Lemma treeify_bindings l : bindings (@treeify elt l) = l.
+Proof.
+ assert (H := @treeify_aux_spec (plength l) true l).
+ unfold treeify. destruct treeify_aux as (t,acc); simpl in *.
+ destruct H as (H,H'). { now rewrite plength_spec. }
+ subst l. rewrite plength_spec, app_length, <- bindings_cardinal in *.
+ destruct acc.
+ * now rewrite app_nil_r.
+ * exfalso. revert H. simpl.
+   rewrite Nat.add_succ_r, Nat.add_comm.
+   apply Nat.succ_add_discr.
+Qed.
+
+Lemma treeify_mapsto x v l : MapsTo x v (treeify l) <-> InA O.eqke (x,v) l.
+Proof.
+ intros. now rewrite <- bindings_mapsto, treeify_bindings.
+Qed.
+
+(* Todo : migrate this section elsewhere someday... *)
+
+Section MoreOnSortA.
+Context {A} eqA `{Equivalence A eqA}.
+Context ltA `{StrictOrder A ltA} `{!Proper (eqA==>eqA==>iff) ltA}.
+
+Lemma SortA_app (l1 l2 : list A) :
+ sort ltA (l1++l2) <->
+ sort ltA l1 /\ sort ltA l2 /\
+  forall a1 a2, List.In a1 l1 -> List.In a2 l2 -> ltA a1 a2.
+Proof.
+ split.
+ { induction l1 as [|a1 l1 IHl1].
+   - easy.
+   - simpl. inversion_clear 1 as [ | ? ? Hs Hhd ].
+     destruct (IHl1 Hs) as (H1 & H2 & H3); clear IHl1.
+     repeat split.
+     * constructor; auto.
+       destruct l1; simpl in *; auto; inversion_clear Hhd; auto.
+     * trivial.
+     * intros b1 b2 [->|Hb1] Hb2; eauto.
+       eapply SortA_InfA_InA with (eqA:=eqA)(l:=l1++l2); auto.
+       rewrite InA_app_iff. right. apply In_InA; ok. }
+ { intros (U & V & W); eapply SortA_app; eauto.
+   intros x y. rewrite !InA_alt.
+   intros (x' & -> & Hx) (y' & -> & Hy); auto. }
+Qed.
+
+End MoreOnSortA.
+
+(** Apart predicate on lists *)
+
+Section ApartList.
+Context {A B : Type}.
+Implicit Types lA : klist A.
+Implicit Types lB : klist B.
+
+Definition ApartL lA lB :=
+ forall ka kb, List.In ka lA -> List.In kb lB -> ka#1 < kb#1.
+
+Lemma ApartL_rev lA lB : ApartL (rev lA) lB <-> ApartL lA lB.
+Proof.
+ unfold ApartL. now setoid_rewrite <- in_rev.
+Qed.
+
+Lemma ApartL_appl lA lA' lB :
+ ApartL (lA++lA') lB <-> ApartL lA lB /\ ApartL lA' lB.
+Proof.
+ unfold ApartL. setoid_rewrite in_app_iff; firstorder.
+Qed.
+
+Lemma ApartL_appr lA lB lB' :
+ ApartL lA (lB++lB') <-> ApartL lA lB /\ ApartL lA lB'.
+Proof.
+ unfold ApartL. setoid_rewrite in_app_iff; firstorder.
+Qed.
+
+Lemma ApartL_consl ka lA lB :
+ ApartL (ka::lA) lB <-> ApartL [ka] lB /\ ApartL lA lB.
+Proof.
+ apply (ApartL_appl [ka]).
+Qed.
+
+Lemma ApartL_consr kb lA lB :
+ ApartL lA (kb::lB) <-> ApartL lA [kb] /\ ApartL lA lB.
+Proof.
+ apply (ApartL_appr lA [kb]).
+Qed.
+
+End ApartList.
+
+Lemma ApartL_eqk_l {A B B'} (lA : klist A) (kb:key*B) (kb':key*B') :
+ ApartL [kb] lA -> K.eq (kb#1) (kb'#1) -> ApartL [kb'] lA.
+Proof.
+ unfold ApartL. simpl. intros AP E (k,b') (k',a) [<-|[ ]] Hy; simpl.
+ rewrite <-E. apply (AP kb (k',a)); auto.
+Qed.
+
+Lemma ApartL_ltk_l {A B B'} (lA : klist A) (kb:key*B) (kb':key*B') :
+ ApartL [kb] lA -> K.lt (kb'#1) (kb#1) -> ApartL [kb'] lA.
+Proof.
+ unfold ApartL. simpl. intros AP LT (k,b') (k',a) [<-|[ ]] Hy; simpl.
+ rewrite LT. apply (AP kb (k',a)); auto.
+Qed.
+
+Lemma ApartL_eqk_r {A B B'} (lA : klist A) (kb:key*B) (kb':key*B') :
+ ApartL lA [kb] -> K.eq (kb#1) (kb'#1) -> ApartL lA [kb'].
+Proof.
+ unfold ApartL. simpl. intros AP E (k,a) (k',b') Hx [<-|[ ]]; simpl.
+ rewrite <-E. apply (AP (k,a) kb); auto.
+Qed.
+
+Lemma ApartL_ltk_r {A B B'} (lA : klist A) (kb:key*B) (kb':key*B') :
+ ApartL lA [kb] -> K.lt (kb#1) (kb'#1) -> ApartL lA [kb'].
+Proof.
+ unfold ApartL. simpl. intros AP LT (k,a) (k',b') Hx [<-|[ ]]; simpl.
+ rewrite <-LT. apply (AP (k,a) kb); auto.
+Qed.
+
+Lemma sort_app_key (l l' : klist elt) :
+ sort O.ltk (l++l') <-> sort O.ltk l /\ sort O.ltk l' /\ ApartL l l'.
+Proof.
+ apply SortA_app with (eqA:=O.eqk)(ltA:=O.ltk); ok.
+Qed.
+
+Lemma sort_cons_key p (l : klist elt) :
+ sort O.ltk (p::l) <-> sort O.ltk l /\ ApartL [p] l.
+Proof.
+ rewrite (sort_app_key [p] l). firstorder.
+Qed.
+
+Lemma bindings_above x (e:elt) (m:t elt) :
+  x >> m <-> ApartL (bindings m) [(x,e)].
+Proof.
+ rewrite above_alt. unfold ApartL. simpl. split.
+ - intros H p q Hp [<-|[ ]]. simpl. apply H.
+   rewrite <- In_alt. exists (p#2). rewrite <- bindings_mapsto.
+   apply In_InA; ok. now destruct p.
+ - intros H y. rewrite <-In_alt. intros (v,M).
+   rewrite <- bindings_mapsto, InA_alt in M.
+   destruct M as ((y',v') & (E,E') & IN). compute in E, E'.
+   subst v'. rewrite E. apply (H (y',v) (x,e)); auto.
+Qed.
+
+Lemma bindings_below x (e:elt) (m:t elt) :
+  x << m <-> ApartL [(x,e)] (bindings m).
+Proof.
+ rewrite below_alt. unfold ApartL. simpl. split.
+ - intros H p q [<-|[ ]] Hq. simpl. apply H.
+   rewrite <- In_alt. exists (q#2). rewrite <- bindings_mapsto.
+   apply In_InA; ok. now destruct q.
+ - intros H y. rewrite <-In_alt. intros (v,M).
+   rewrite <- bindings_mapsto, InA_alt in M.
+   destruct M as ((y',v') & (E,E') & IN). compute in E, E'.
+   subst v'. rewrite E. apply (H (x,e) (y',v)); auto.
+Qed.
+
+Lemma bindings_sort_ok (m:t elt) : sort O.ltk (bindings m) <-> Ok m.
+Proof.
+ split; auto using bindings_sort.
+ induction m as [|c l IHl x v r IHr].
+ - unfold bindings. simpl. firstorder.
+ - rewrite bindings_node.
+   rewrite sort_app_key, sort_cons_key, ApartL_consr.
+   rewrite <- bindings_above, <- bindings_below. intuition; ok.
+Qed.
+
+Instance treeify_ok l : sort O.ltk l -> Ok (@treeify elt l).
+Proof.
+ intros. apply bindings_sort_ok. rewrite treeify_bindings; auto.
+Qed.
+
+End Elt.
+
+Definition Keqb x y :=
+  match K.compare x y with
+  | Eq => true
+  | _ => false
+  end.
+
+Lemma Keqb_spec x y : reflect (K.eq x y) (Keqb x y).
+Proof.
+ unfold Keqb. destruct (K.compare x y) eqn:E; constructor.
+ - revert E. now case K.compare_spec.
+ - revert E. case K.compare_spec; easy || order.
+ - revert E. case K.compare_spec; easy || order.
+Qed.
+
+Definition oelse {A} (o o' : option A) :=
+ match o with
+ | None => o'
+ | _ => o
+ end.
+
+Definition obind {A B} (o:option A) (f:A->option B) :=
+  match o with Some a => f a | None => None end.
+
+Lemma findA_app {A B} (h:A->bool) (l l' : list (A*B)) :
+  findA h (l++l') = oelse (findA h l) (findA h l').
+Proof.
+ induction l as [|(a,b) l IH]; simpl; auto.
+ rewrite IH. destruct (h a); auto.
+Qed.
+
+Lemma findA_inA {elt} x e (l : klist elt) :
+ findA (Keqb x) l = Some e -> InA O.eqke (x,e) l.
+Proof.
+ induction l as [|(k,v) l IH]; simpl; try easy.
+ case Keqb_spec; intro E; auto. intros [= ->]; auto.
+Qed.
+
+Lemma findA_inA_iff {elt} x e (l : klist elt) : sort O.ltk l ->
+ (findA (Keqb x) l = Some e <-> InA O.eqke (x,e) l).
+Proof.
+ intros Sl. split; [apply findA_inA| ]. revert Sl.
+ induction l as [|(k,v) l IH]; simpl; try easy.
+ inversion_clear 1. rewrite InA_cons. intros [(E,E')|IN].
+ - compute in E, E'. subst.
+   case Keqb_spec; intros; auto || order.
+ - case Keqb_spec; intros; auto.
+   assert (LT : O.ltk (k,v) (x,e))
+     by (eapply SortA_InfA_InA with (eqA:=O.eqke); ok).
+   compute in LT. order.
+Qed.
+
+Lemma findA_find {elt} x (m : t elt) `{!Ok m} :
+ findA (Keqb x) (bindings m) = find x m.
+Proof.
+ apply eq_option_alt. intro e.
+ rewrite findA_inA_iff by now apply bindings_sort.
+ rewrite find_spec by auto.
+ apply bindings_mapsto.
+Qed.
+
+Section Mapo.
+Variable elt elt' : Type.
+Variable f : key -> elt -> option elt'.
+
+Lemma mapoL_sorted (l : klist elt) acc :
+ sort O.ltk (rev l) -> sort O.ltk acc -> ApartL l acc ->
+ sort O.ltk (mapoL f l acc).
+Proof.
+ revert acc.
+ induction l as [|(k,e) l IH]; simpl; auto.
+ intros acc Sl Sacc AP.
+ rewrite sort_app_key in Sl; ok. destruct Sl as (Sl & _ & AP').
+ rewrite ApartL_rev, ApartL_consr in AP'. destruct AP' as (AP1',AP').
+ rewrite ApartL_consl in AP. destruct AP as (AP1,AP).
+ apply IH; clear IH; simpl; auto; destruct (f k e); simpl; auto.
+ - apply sort_cons_key. eauto using ApartL_eqk_l.
+ - apply ApartL_consr. eauto using ApartL_eqk_r.
+Qed.
+
+Global Instance mapo_ok m `{!Ok m} : Ok (mapo f m).
+Proof.
+ unfold mapo. apply treeify_ok. apply mapoL_sorted; simpl; auto.
+ - rewrite rev_bindings_rev, rev_involutive. now apply bindings_sort.
+ - inversion 2.
+Qed.
+
+Lemma mapoL_find l acc x :
+ sort O.ltk (rev l) ->
+ exists y : K.t,
+    y == x /\
+    findA (Keqb x) (mapoL f l acc) =
+     oelse (obind (findA (Keqb x) (rev l)) (f y)) (findA (Keqb x) acc).
+Proof.
+ revert acc.
+ induction l as [|(k,e) l IH]; simpl; intros acc Sl.
+ - now exists x.
+ - rewrite sort_app_key in Sl. destruct Sl as (Sl & _ & AP).
+   rewrite ApartL_rev in AP.
+   destruct (IH (ocons k (f k e) acc) Sl) as (y & Hy & E). clear IH.
+   setoid_rewrite findA_app. setoid_rewrite E. clear E.
+   destruct (findA (Keqb x) (rev l)) eqn:El; simpl in *; auto.
+   + exists y; split; auto.
+     destruct (f y e0); simpl; auto.
+     destruct (f k e); simpl; auto.
+     case Keqb_spec; auto. intros.
+     apply findA_inA in El. rewrite InA_rev in El.
+     apply InA_alt in El.
+     destruct El as ((x',e') & (Hx',_) & IN).
+     compute in Hx'.
+     enough (x' < k) by order.
+     apply (AP (x',e') (k,e)); simpl; auto.
+   + clear l Sl AP El.
+     destruct (f k e) eqn:Fk; simpl.
+     * case Keqb_spec; [exists k | exists y]; simpl; now rewrite ?Fk.
+     * case Keqb_spec; [exists k | exists y]; simpl; now rewrite ?Fk.
+Qed.
+
+Lemma mapoL_mapsto l acc x v' :
+ InA O.eqke (x,v') (mapoL f l acc) <->
+ (exists y v, K.eq y x /\ List.In (y,v) l /\ f y v = Some v') \/
+  InA O.eqke (x,v') acc.
+Proof.
+ revert acc.
+ induction l as [|(k,e) l IH]; simpl; intros.
+ - firstorder.
+ - destruct (f k e) eqn:Hf; simpl in *; rewrite IH; clear IH; auto.
+   rewrite ?InA_cons.
+   + firstorder; try red in H; try red in H0; simpl in *; subst.
+     * left. exists k, e; auto.
+     * injection H0 as <- <-. right; left. compute; split; auto.
+       congruence.
+   + firstorder. injection H0 as <- <-. congruence.
+Qed.
+
+Lemma mapo_mapsto m x (v':elt') :
+  MapsTo x v' (mapo f m) ->
+   exists y v, K.eq y x /\ MapsTo x v m /\ f y v = Some v'.
+Proof.
+ unfold mapo.
+ rewrite treeify_mapsto, mapoL_mapsto, InA_nil; auto.
+ intros [(y & v & E & IN & Hf)|[ ]].
+ rewrite rev_bindings_rev, <-In_rev in IN.
+ exists y, v. repeat split; auto. apply bindings_mapsto.
+ rewrite InA_alt. exists (y, v). split; auto.
+Qed.
+
+Lemma mapo_in m x :
+ x ∈ (mapo f m) ->
+  exists y d, K.eq y x /\ MapsTo x d m /\ f y d <> None.
+Proof.
+ rewrite <- In_alt. intros (v',H).
+ apply mapo_mapsto in H. destruct H as (y & v & E & M & Hf).
+ exists y, v; repeat split; congruence.
+Qed.
+
+Lemma mapo_find m x `{!Ok m} :
+  exists y, K.eq y x /\
+            find x (mapo f m) = obind (find x m) (f y).
+Proof.
+ assert (Ok (mapo f m)) by ok.
+ destruct (@mapoL_find (rev_bindings m) nil x) as (y & Hy & EQ).
+ - rewrite rev_bindings_rev, rev_involutive; now apply bindings_sort.
+ - exists y; split; auto.
+   unfold mapo in *. rewrite <- !findA_find; auto.
+   rewrite treeify_bindings, EQ. simpl. clear EQ.
+   rewrite rev_bindings_rev, rev_involutive. now destruct obind.
+Qed.
+
+End Mapo.
+
+Section Merge.
+Variable elt elt' elt'' : Type.
+Implicit Type f : key -> option elt -> option elt' -> option elt''.
+
+Lemma mergeL_sorted f l l' acc :
+ sort O.ltk (rev l) -> sort O.ltk (rev l') -> sort O.ltk acc ->
+ ApartL l acc -> ApartL l' acc ->
+ sort O.ltk (mergeL f l l' acc).
+Proof.
+ revert l' acc.
+ induction l as [|(x,e) l IHl].
+ - simpl. intros. apply mapoL_sorted; auto.
+ - induction l' as [|(x',e') l' IHl'].
+   + intros. apply mapoL_sorted; auto.
+   + intros acc Sl Sl' Sacc AP AP'.
+     simpl; destmatch.
+     * intros E.
+       simpl in Sl, Sl'.
+       apply sort_app_key in Sl. destruct Sl as (Sl & _ & APl).
+       apply sort_app_key in Sl'. destruct Sl' as (Sl' & _ & APl').
+       rewrite ApartL_rev in APl. rewrite ApartL_rev in APl'.
+       rewrite ApartL_consl in AP. destruct AP as (AP1,AP).
+       rewrite ApartL_consl in AP'. destruct AP' as (AP1',AP').
+       apply IHl; clear IHl IHl'; auto; destruct f; simpl; auto.
+       { apply sort_cons_key. eauto using ApartL_eqk_l. }
+       { rewrite ApartL_consr. eauto using ApartL_eqk_r. }
+       { rewrite ApartL_consr. eauto using ApartL_eqk_r. }
+     * intros LT.
+       change (Sorted O.ltk (mergeL f ((x,e)::l) l'
+                             (ocons x' (f x' None (Some e')) acc))).
+       simpl in Sl'.
+       apply sort_app_key in Sl'. destruct Sl' as (Sl' & _ & APl').
+       rewrite ApartL_rev in APl'.
+       rewrite ApartL_consl in AP'. destruct AP' as (AP1',AP').
+       apply IHl'; clear IHl IHl'; auto; destruct f; simpl; auto.
+       { apply sort_cons_key. eauto using ApartL_eqk_l. }
+       { rewrite ApartL_consr. split; auto.
+         rewrite ApartL_consl. split.
+         - intros (?,?) (?,?). compute. intuition congruence.
+         - simpl in Sl. rewrite sort_app_key, ApartL_rev in Sl.
+           destruct Sl as (_ & _ & ?). eauto using ApartL_ltk_r. }
+       { rewrite ApartL_consr. eauto using ApartL_eqk_r. }
+     * intros LT.
+       simpl in Sl.
+       apply sort_app_key in Sl. destruct Sl as (Sl & _ & APl).
+       rewrite ApartL_rev in APl.
+       rewrite ApartL_consl in AP. destruct AP as (AP1,AP).
+       apply IHl; clear IHl IHl'; auto; destruct f; simpl; auto.
+       { apply sort_cons_key. eauto using ApartL_eqk_l. }
+       { rewrite ApartL_consr. eauto using ApartL_eqk_r. }
+       { rewrite ApartL_consr. split; auto.
+         rewrite ApartL_consl. split.
+         - intros (?,?) (?,?). compute. intuition congruence.
+         - simpl in Sl'. rewrite sort_app_key, ApartL_rev in Sl'.
+           destruct Sl' as (_ & _ & ?). eauto using ApartL_ltk_r. }
+Qed.
+
+Global Instance merge_ok f m m' `{!Ok m, !Ok m'} : Ok (merge f m m').
+Proof.
+apply treeify_ok, mergeL_sorted; auto;
+ rewrite ?rev_bindings_rev, ?rev_involutive;
+ now apply bindings_sort || firstorder.
+Qed.
+
+Lemma mergeL_in f l l' acc x :
+ (exists v, InA O.eqke (x,v) (mergeL f l l' acc)) ->
+    (exists v, InA O.eqke (x,v) l) \/
+    (exists v, InA O.eqke (x,v) l') \/
+    (exists v, InA O.eqke (x,v) acc).
+Proof.
+ revert l' acc.
+ induction l as [|(y,e) l IHl].
+ - simpl. intros l' acc (v,H). right.
+   apply mapoL_mapsto in H.
+   destruct H as [(y & v' & E & IN & _)|H].
+   + left; exists v'. rewrite InA_alt. exists (y,v'); split; auto.
+   + firstorder.
+ - induction l' as [|(y',e') l' IHl'].
+   + intros acc (v,H). apply mapoL_mapsto in H; simpl in *.
+     destruct H as [(y' & v' & E & [[= <- <-]|IN] & _)|H].
+     * left. exists e; eauto.
+     * left. exists v'. rewrite InA_cons. right. rewrite InA_alt.
+       exists (y',v'); auto.
+     * firstorder.
+   + intros acc. simpl; destmatch.
+     * intros E H. apply IHl in H; clear IHl IHl'.
+       setoid_rewrite InA_cons.
+       firstorder.
+       destruct f; simpl in *; [ | firstorder].
+       rewrite InA_cons in H; destruct H as [H|H]; [ | firstorder ].
+       compute in H. destruct H as (H,_).
+       left. exists e. now left.
+     * intros LT H.
+       change (exists v,
+               InA O.eqke (x,v) (mergeL f ((y,e)::l) l'
+                                  (ocons y' (f y' None (Some e')) acc)))
+       in H.
+       apply IHl' in H; clear IHl IHl'.
+       setoid_rewrite InA_cons at 2.
+       firstorder.
+       destruct f; simpl in *; [ | firstorder].
+       rewrite InA_cons in H; destruct H as [H|H]; [ | firstorder ].
+       compute in H. destruct H as (H,_).
+       right; left. exists e'. now left.
+     * intros LT H.
+       apply IHl in H; clear IHl IHl'.
+       setoid_rewrite InA_cons at 1.
+       firstorder.
+       destruct f; simpl in *; [ | firstorder].
+       rewrite InA_cons in H; destruct H as [H|H]; [ | firstorder ].
+       compute in H. destruct H as (H,_).
+       left. exists e. now left.
+Qed.
+
+Lemma merge_spec2 f m m' x :
+  In x (merge f m m') -> In x m \/ In x m'.
+Proof.
+ unfold merge.
+ rewrite <- !In_alt. unfold In0. setoid_rewrite treeify_mapsto.
+ intros H. apply mergeL_in in H. destruct H as [(v,H)|[(v,H)|(v,H)]].
+ - left. exists v. rewrite rev_bindings_rev, InA_rev in H.
+   now apply bindings_mapsto.
+ - right. exists v. rewrite rev_bindings_rev, InA_rev in H.
+   now apply bindings_mapsto.
+ - now rewrite InA_nil in H.
+Qed.
+
+Lemma mergeL_find f l l' acc x :
+ (forall k, f k None None = None) ->
+ sort O.ltk (rev l) ->
+ sort O.ltk (rev l') ->
+ exists y, K.eq y x /\
+  findA (Keqb x) (mergeL f l l' acc) =
+    oelse (f y (findA (Keqb x) (rev l)) (findA (Keqb x) (rev l')))
+          (findA (Keqb x) acc).
+Proof.
+ intros Hf.
+ revert l' acc.
+ induction l as [|(y,e) l IHl].
+ - simpl. intros l' acc _ Sl'.
+   destruct (@mapoL_find _ _ (fun k v' => f k None (Some v')) l' acc x Sl')
+     as (y & Hy & EQ).
+   exists y; split; auto; rewrite EQ; clear EQ.
+   destruct findA; simpl; rewrite ?Hf; auto.
+ - induction l' as [|(y',e') l' IHl'].
+   + intros acc Sl _. clear IHl.
+     destruct (@mapoL_find _ _ (fun k v => f k (Some v) None) _ acc x Sl)
+       as (z & Hz & EQ).
+     exists z; split; auto. cbn - [mapoL]. rewrite EQ; clear EQ.
+     simpl. destruct findA; simpl; rewrite ?Hf; auto.
+   + intros acc Sl Sl'.
+     simpl mergeL. destmatch; intro E.
+     * simpl in Sl, Sl'. rewrite sort_app_key in Sl, Sl'.
+       destruct Sl as (Sl & _ & AP). destruct Sl' as (Sl' & _ & AP').
+       destruct (IHl l' (ocons y (f y (Some e) (Some e')) acc))
+        as (z & Hz & EQ); auto.
+       setoid_rewrite EQ. clear IHl IHl' EQ.
+       simpl. setoid_rewrite findA_app; simpl.
+       destruct findA eqn:INl.
+       ** exists z; split; auto.
+          assert (x < y).
+          { apply findA_inA in INl. apply InA_alt in INl.
+            destruct INl as ((x',e0') & (Hx',_) & INl).
+            compute in Hx'. rewrite Hx'.
+            apply (AP (x',e0') (y,e)); simpl; auto. }
+          destruct (findA _ (rev l')) eqn:INl'; simpl.
+          *** destruct (f z _ _); simpl; auto.
+              destruct (f y _ _); simpl; auto.
+              case Keqb_spec; auto || order.
+          *** case Keqb_spec; auto; try order. intros.
+              destruct (f z _ _); simpl; auto.
+              destruct (f y _ _); simpl; auto.
+              case Keqb_spec; auto || order.
+       ** clear INl.
+          destruct (findA _ (rev l')) eqn:INl'; simpl.
+          *** exists z; split; auto.
+              assert (x < y').
+              { apply findA_inA in INl'. apply InA_alt in INl'.
+                destruct INl' as ((x',e0') & (Hx',_) & INl').
+                compute in Hx'. rewrite Hx'.
+                apply (AP' (x',e0') (y',e')); simpl; auto. }
+              case Keqb_spec; auto; try order. intros.
+              destruct (f z _ _); simpl; auto.
+              destruct (f y _ _); simpl; auto.
+              case Keqb_spec; auto || order.
+          *** clear INl'. rewrite Hf. simpl.
+              destruct (f y _ _) eqn:Fy; simpl;
+               case Keqb_spec; intros;
+                case Keqb_spec; intros; try order;
+                 try setoid_rewrite Hf; firstorder;
+                 exists y; now rewrite Fy.
+     * change
+         (exists y0, y0 == x /\
+           findA (Keqb x)
+                 (mergeL f ((y,e)::l) l'
+                   (ocons y' (f y' None (Some e')) acc)) =
+           oelse
+             (f y0 (findA (Keqb x) (rev ((y, e) :: l)))
+                (findA (Keqb x) (rev ((y', e') :: l'))))
+             (findA (Keqb x) acc)).
+       simpl in Sl'. rewrite sort_app_key in Sl'.
+       destruct Sl' as (Sl' & _ & AP').
+       destruct (IHl' (ocons y' (f y' None (Some e')) acc))
+        as (z & Hz & EQ); auto.
+       setoid_rewrite EQ. clear IHl IHl' EQ.
+       remember ((y,e)::l) as l0.
+       simpl. setoid_rewrite findA_app.
+       destruct findA eqn:INl.
+       ** exists z; split; auto.
+          assert (x < y').
+          { apply findA_inA in INl. apply InA_alt in INl.
+            destruct INl as ((x',e0') & (Hx',_) & INl).
+            compute in Hx'. rewrite Hx'.
+            rewrite Heql0 in *. simpl in *.
+            rewrite sort_app_key in Sl.
+            destruct Sl as (Sl & _ & AP).
+            rewrite in_app_iff in INl. destruct INl.
+            - rewrite <- E. apply (AP (x',e0') (y,e)); simpl; auto.
+            - simpl in H. destruct H as [[= <- _]|[  ]]; auto. }
+          destruct (findA _ (rev l')) eqn:INl'; simpl.
+          *** destruct (f z _ _); simpl; auto.
+              destruct (f y' _ _); simpl; auto.
+              case Keqb_spec; auto || order.
+          *** case Keqb_spec; auto; try order. intros.
+              destruct (f z _ _); simpl; auto.
+              destruct (f y' _ _); simpl; auto.
+              case Keqb_spec; auto || order.
+       ** clear INl.
+          destruct (findA _ (rev l')) eqn:INl'; simpl.
+          *** exists z; split; auto.
+              assert (x < y').
+              { apply findA_inA in INl'. apply InA_alt in INl'.
+                destruct INl' as ((x',e0') & (Hx',_) & INl').
+                compute in Hx'. rewrite Hx'.
+                apply (AP' (x',e0') (y',e')); simpl; auto. }
+              destruct (f z _ _); simpl; auto.
+              destruct (f y' _ _); simpl; auto.
+              case Keqb_spec; auto || order.
+          *** clear INl'. rewrite Hf. simpl.
+              destruct (f y' _ _) eqn:Fy'; simpl;
+               case Keqb_spec; intros;
+                 try setoid_rewrite Hf; firstorder;
+                 exists y'; now rewrite Fy'.
+     * simpl in Sl. rewrite sort_app_key in Sl.
+       destruct Sl as (Sl & _ & AP).
+       destruct (IHl ((y',e')::l') (ocons y (f y (Some e) None) acc))
+        as (z & Hz & EQ); auto.
+       setoid_rewrite EQ. clear IHl IHl' EQ.
+       remember ((y',e')::l') as l0'.
+       simpl. setoid_rewrite findA_app.
+       destruct findA eqn:INl.
+       ** exists z; split; auto.
+          assert (x < y).
+          { apply findA_inA in INl. apply InA_alt in INl.
+            destruct INl as ((x',e0') & (Hx',_) & INl).
+            compute in Hx'. rewrite Hx'.
+            apply (AP (x',e0') (y,e)); simpl; auto. }
+          destruct (findA _ (rev l0')) eqn:INl'; simpl.
+          *** destruct (f z _ _); simpl; auto.
+              destruct (f y _ _); simpl; auto.
+              case Keqb_spec; auto || order.
+          *** destruct (f z _ _); simpl; auto.
+              destruct (f y _ _); simpl; auto.
+              case Keqb_spec; auto || order.
+       ** clear INl.
+          destruct (findA _ (rev l0')) eqn:INl'; simpl.
+          *** exists z; split; auto.
+              assert (x < y).
+              { apply findA_inA in INl'. apply InA_alt in INl'.
+                destruct INl' as ((x',e0') & (Hx',_) & INl').
+                compute in Hx'. rewrite Hx'.
+                rewrite Heql0' in *. simpl in *.
+                rewrite sort_app_key in Sl'.
+                destruct Sl' as (Sl' & _ & AP').
+                rewrite in_app_iff in INl'. destruct INl'.
+                - rewrite <- E. apply (AP' (x',e0') (y',e')); simpl; auto.
+                - simpl in H. destruct H as [[= <- _]|[  ]]; auto. }
+              case Keqb_spec; auto; try order. intros.
+              destruct (f z _ _); simpl; auto.
+              destruct (f y _ _); simpl; auto.
+              case Keqb_spec; auto || order.
+          *** clear INl'. rewrite Hf. simpl.
+              destruct (f y _ _) eqn:Fy; simpl;
+               case Keqb_spec; intros;
+                 try setoid_rewrite Hf; firstorder;
+                 exists y; now rewrite Fy.
+Qed.
+
+Lemma merge_spec1n f m m' x `{!Ok m, !Ok m'} :
+ (forall k, f k None None = None) ->
+ exists y, K.eq y x /\
+           find x (merge f m m') = f y (find x m) (find x m').
+Proof.
+ intros Hf.
+ assert (Ok (merge f m m')) by ok.
+ destruct (@mergeL_find f (rev_bindings m) (rev_bindings m') nil x)
+   as (y & Hy & EQ); auto.
+ - rewrite rev_bindings_rev, rev_involutive; now apply bindings_sort.
+ - rewrite rev_bindings_rev, rev_involutive; now apply bindings_sort.
+ - exists y; split; auto.
+   unfold merge in *. rewrite <- !findA_find; auto.
+   rewrite treeify_bindings, EQ. simpl. clear EQ.
+   rewrite rev_bindings_rev, rev_involutive.
+   rewrite rev_bindings_rev, rev_involutive.
+   now destruct f.
+Qed.
+
+Lemma merge_spec1 f m m' x `{!Ok m, !Ok m'} :
+ (In x m \/ In x m') ->
+ exists y, K.eq y x /\
+           find x (merge f m m') = f y (find x m) (find x m').
+Proof.
+ set (g := fun x o o' => match o,o' with None, None => None
+                                        | _,_ => f x o o' end).
+ destruct (@merge_spec1n g m m' x) as (y & Hy & EQ); auto.
+ change (merge f) with (merge g).
+ exists y; split; auto. rewrite EQ.
+ destruct (find x m) eqn:F; simpl; auto.
+ destruct (find x m') eqn:F'; simpl; auto.
+ rewrite not_find_iff in F, F'; intuition.
+Qed.
+
+End Merge.
+End Raw.
+
+(** * Encapsulation
+
+   Now, in order to really provide a functor implementing [S], we
+   need to encapsulate everything into a type of binary search trees. *)
+
+Module Make (K: OrderedType) <: S K.
+
+ Module Import Raw := Raw K.
+
+ Record tree (elt:Type) :=
+  Mk {this :> Raw.tree elt; is_ok : Ok this}.
+
+ Existing Instance is_ok.
+ Local Arguments Mk {elt} this {is_ok}.
+
+ Definition t := tree.
+ Definition key := K.t.
+
+ Section Elt.
+ Variable elt elt' elt'': Type.
+
+ Implicit Types m : t elt.
+ Implicit Types x y : key.
+ Implicit Types e : elt.
+
+ Definition empty : t elt := Mk (empty elt).
+ Definition is_empty m : bool := is_empty m.
+ Definition add x e m : t elt := Mk (add x e m).
+ Definition remove x m : t elt := Mk (remove x m).
+ Definition mem x m : bool := mem x m.
+ Definition find x m : option elt := Raw.find x m.
+ Definition map f m : t elt' := Mk (map f m).
+ Definition mapi (f:key->elt->elt') m : t elt' := Mk (mapi f m).
+ Definition merge f m (m':t elt') : t elt'' := Mk (merge f m m').
+ Definition bindings m : list (key*elt) := bindings m.
+ Definition cardinal m := cardinal m.
+ Definition fold {A} (f:key->elt->A->A) m i := fold f m i.
+ Definition equal cmp m m' : bool := equal cmp m m'.
+
+ Definition MapsTo x e m : Prop := MapsTo x e m.
+ Definition In x m : Prop := In0 x m.
+
+ Definition eq_key : (key*elt) -> (key*elt) -> Prop := @O.eqk elt.
+ Definition eq_key_elt : (key*elt) -> (key*elt) -> Prop := @O.eqke elt.
+ Definition lt_key : (key*elt) -> (key*elt) -> Prop := @O.ltk elt.
+
+ Instance MapsTo_compat :
+   Proper (K.eq==>Logic.eq==>Logic.eq==>iff) MapsTo.
+ Proof.
+   intros k k' Hk e e' <- m m' <-. unfold MapsTo; simpl. now rewrite Hk.
+ Qed.
+
+ Lemma find_spec m x e : find x m = Some e <-> MapsTo x e m.
+ Proof. apply find_spec; autok. Qed.
+
+ Lemma mem_spec m x : mem x m = true <-> In x m.
+ Proof. unfold In, mem; rewrite In_alt. apply mem_spec; autok. Qed.
+
+ Lemma empty_spec x : find x empty = None.
+ Proof. apply empty_spec. Qed.
+
+ Lemma is_empty_spec m : is_empty m = true <-> forall x, find x m = None.
+ Proof. apply is_empty_spec. Qed.
+
+ Lemma add_spec1 m x e : find x (add x e m) = Some e.
+ Proof. apply add_spec1; autok. Qed.
+ Lemma add_spec2 m x y e : ~ K.eq x y -> find y (add x e m) = find y m.
+ Proof. apply add_spec2; autok. Qed.
+
+ Lemma remove_spec1 m x : find x (remove x m) = None.
+ Proof. apply remove_spec1; autok. Qed.
+ Lemma remove_spec2 m x y : ~K.eq x y -> find y (remove x m) = find y m.
+ Proof. apply remove_spec2; autok. Qed.
+
+ Lemma bindings_spec1 m x e :
+   InA eq_key_elt (x,e) (bindings m) <-> MapsTo x e m.
+ Proof. apply bindings_mapsto. Qed.
+
+ Lemma bindings_spec2 m : sort lt_key (bindings m).
+ Proof. apply bindings_sort; autok. Qed.
+
+ Lemma bindings_spec2w m : NoDupA eq_key (bindings m).
+ Proof. apply bindings_nodup; autok. Qed.
+
+ Lemma fold_spec m {A} (i : A) (f : key -> elt -> A -> A) :
+   fold f m i = fold_left (fun a p => f (fst p) (snd p) a) (bindings m) i.
+ Proof. apply fold_spec; autok. Qed.
+
+ Lemma cardinal_spec m : cardinal m = length (bindings m).
+ Proof. apply bindings_cardinal. Qed.
+
+ Definition Equal m m' := forall y, find y m = find y m'.
+ Definition Eqdom (m m':t elt) := forall y, In y m <-> In y m'.
+ Definition Equiv (R:elt->elt->Prop) m m' :=
+  Eqdom m m' /\ (forall k e e', MapsTo k e m -> MapsTo k e' m' -> R e e').
+ Definition Equivb cmp := Equiv (Cmp cmp).
+
+ Lemma Equivb_Equivb cmp m m' :
+  Equivb cmp m m' <-> Raw.Equivb cmp m m'.
+ Proof.
+ unfold Equivb, Equiv, Raw.Equivb, In. intuition.
+ intros k. rewrite <- !In_alt. apply H0.
+ intros k. unfold In; rewrite !In_alt. apply H0.
+ Qed.
+
+ Lemma equal_spec m m' cmp :
+   equal cmp m m' = true <-> Equivb cmp m m'.
+ Proof. rewrite Equivb_Equivb. apply equal_Equivb; apply is_ok. Qed.
+
+ End Elt.
+
+ Lemma map_spec {elt elt'} (f:elt->elt') m x :
+   find x (map f m) = option_map f (find x m).
+ Proof. apply map_spec. Qed.
+
+ Lemma mapi_spec {elt elt'} (f:key->elt->elt') m x :
+   exists y:key, K.eq y x /\ find x (mapi f m) = option_map (f y) (find x m).
+ Proof. apply mapi_spec. Qed.
+
+ Lemma merge_spec1 {elt elt' elt''}
+       (f:key->option elt->option elt'->option elt'') m m' x :
+   In x m \/ In x m' ->
+   exists y:key, K.eq y x /\
+                 find x (merge f m m') = f y (find x m) (find x m').
+ Proof. unfold In. rewrite !In_alt. apply merge_spec1; autok. Qed.
+
+ Lemma merge_spec2 {elt elt' elt''}
+       (f:key -> option elt->option elt'->option elt'') m m' x :
+   In x (merge f m m') -> In x m \/ In x m'.
+ Proof. unfold In. rewrite !In_alt. apply merge_spec2; autok. Qed.
+
+End Make.
+
+Module Make_ord (K:OrderedType)(D:OrderedType) <: Sord K D.
+  Module Import MapS := Make(K).
+  Module LO := MMaps.OrdList.Make_ord(K)(D).
+  Module Import R := Raw.
+
+  Definition t := MapS.t D.t.
+
+  Definition cmp e e' :=
+   match D.compare e e' with Eq => true | _ => false end.
+
+  (** One step of comparison of bindings *)
+
+  Definition compare_more x1 d1 (cont:R.enumeration D.t -> comparison) e2 :=
+   match e2 with
+    | R.End _ => Gt
+    | R.More x2 d2 r2 e2 =>
+       match K.compare x1 x2 with
+        | Eq => match D.compare d1 d2 with
+                   | Eq => cont (R.cons r2 e2)
+                   | Lt => Lt
+                   | Gt => Gt
+                  end
+        | Lt => Lt
+        | Gt => Gt
+       end
+   end.
+
+  (** Comparison of left tree, middle element, then right tree *)
+
+  Fixpoint compare_cont s1 (cont:R.enumeration D.t -> comparison) e2 :=
+   match s1 with
+    | R.Leaf _ => cont e2
+    | R.Node _ l1 x1 d1 r1 =>
+       compare_cont l1 (compare_more x1 d1 (compare_cont r1 cont)) e2
+   end.
+
+  (** Initial continuation *)
+
+  Definition compare_end (e2:R.enumeration D.t) :=
+   match e2 with R.End _ => Eq | _ => Lt end.
+
+  (** The complete comparison *)
+
+  Definition compare m1 m2 :=
+    compare_cont m1.(this) compare_end (R.cons m2.(this) (R.End _)).
+
+  (** Correctness of this comparison *)
+
+  Definition Cmp c :=
+   match c with
+    | Eq => LO.eq_list
+    | Lt => LO.lt_list
+    | Gt => flip LO.lt_list
+   end.
+
+  Lemma cons_Cmp c x1 x2 d1 d2 l1 l2 :
+   K.eq x1 x2 -> D.eq d1 d2 ->
+   Cmp c l1 l2 -> Cmp c ((x1,d1)::l1) ((x2,d2)::l2).
+  Proof.
+    destruct c; simpl; unfold flip; simpl; intros; case K.compare_spec;
+      auto; try F.order.
+    intros. right. split; auto. now symmetry.
+  Qed.
+  Hint Resolve cons_Cmp.
+
+  Lemma compare_end_Cmp e2 :
+   Cmp (compare_end e2) nil (R.flatten_e e2).
+  Proof.
+   destruct e2; simpl; auto.
+  Qed.
+
+  Lemma compare_more_Cmp x1 d1 cont x2 d2 r2 e2 l :
+    Cmp (cont (R.cons r2 e2)) l (R.bindings r2 ++ R.flatten_e e2) ->
+     Cmp (compare_more x1 d1 cont (R.More x2 d2 r2 e2)) ((x1,d1)::l)
+       (R.flatten_e (R.More x2 d2 r2 e2)).
+  Proof.
+   simpl; case K.compare_spec; simpl;
+   try case D.compare_spec; simpl; unfold flip; simpl; auto;
+   case K.compare_spec; try R.F.order; auto.
+  Qed.
+
+  Lemma compare_cont_Cmp : forall s1 cont e2 l,
+   (forall e, Cmp (cont e) l (R.flatten_e e)) ->
+   Cmp (compare_cont s1 cont e2) (R.bindings s1 ++ l) (R.flatten_e e2).
+  Proof.
+    induction s1 as [|h1 l1 Hl1 x1 d1 r1 Hr1] using R.tree_ind;
+    intros; auto.
+    rewrite R.bindings_node_acc; simpl.
+    apply Hl1; auto. clear e2. intros [|x2 d2 r2 e2].
+    simpl; unfold flip; simpl; auto.
+    apply compare_more_Cmp.
+    rewrite <- Raw.cons_1; auto.
+  Qed.
+
+  Lemma compare_Cmp m1 m2 :
+   Cmp (compare m1 m2) (bindings m1) (bindings m2).
+  Proof.
+    destruct m1 as (s1,H1), m2 as (s2,H2).
+    unfold compare; simpl.
+    rewrite <- (app_nil_r (R.bindings s1)).
+    replace (R.bindings s2) with (R.flatten_e (R.cons s2 (R.End _))) by
+    (rewrite R.cons_1; simpl; rewrite app_nil_r; auto).
+    auto using compare_cont_Cmp, compare_end_Cmp.
+  Qed.
+
+  Definition eq (m1 m2 : t) := LO.eq_list (bindings m1) (bindings m2).
+  Definition lt (m1 m2 : t) := LO.lt_list (bindings m1) (bindings m2).
+
+  Lemma compare_spec m1 m2 : CompSpec eq lt m1 m2 (compare m1 m2).
+  Proof.
+    assert (H := compare_Cmp m1 m2).
+    unfold Cmp in H.
+    destruct (compare m1 m2); auto.
+  Qed.
+
+  (* Proofs about [eq] and [lt] *)
+
+  Definition sbindings (m1 : t) :=
+   LO.MapS.Mk (@R.bindings_sort _ m1 _).
+
+  Definition seq (m1 m2 : t) := LO.eq (sbindings m1) (sbindings m2).
+  Definition slt (m1 m2 : t) := LO.lt (sbindings m1) (sbindings m2).
+
+  Lemma eq_seq : forall m1 m2, eq m1 m2 <-> seq m1 m2.
+  Proof.
+   unfold eq, seq, sbindings, bindings, LO.eq; intuition.
+  Qed.
+
+  Lemma lt_slt : forall m1 m2, lt m1 m2 <-> slt m1 m2.
+  Proof.
+   unfold lt, slt, sbindings, bindings, LO.lt; intuition.
+  Qed.
+
+  Lemma eq_spec m m' : eq m m' <-> MapS.Equivb cmp m m'.
+  Proof.
+  rewrite eq_seq; unfold seq.
+  rewrite Equivb_Equivb.
+  rewrite R.Equivb_bindings. apply LO.eq_spec.
+  Qed.
+
+  Instance eq_equiv : Equivalence eq.
+  Proof.
+    constructor; red; [intros x|intros x y| intros x y z];
+    rewrite !eq_seq; apply LO.eq_equiv.
+  Qed.
+
+  Instance lt_compat : Proper (eq ==> eq ==> iff) lt.
+  Proof.
+    intros m1 m2 H1 m1' m2' H2. rewrite !lt_slt. rewrite eq_seq in *.
+    now apply LO.lt_compat.
+  Qed.
+
+  Instance lt_strorder : StrictOrder lt.
+  Proof.
+    constructor; red; [intros x; red|intros x y z];
+    rewrite !lt_slt; apply LO.lt_strorder.
+  Qed.
+
+End Make_ord.
